pcuic/theories/PCUICLiftSubst.v
@@ -135,29 +135,6 @@ Proof.
 Qed.
 Hint Resolve pair_eq_spec : all. *)
 
-Ltac change_Sk :=
-  repeat match goal with
-    | |- context [S (?x + ?y)] => progress change (S (x + y)) with (S x + y)
-    | |- context [#|?l| + (?x + ?y)] => progress replace (#|l| + (x + y)) with ((#|l| + x) + y) by now rewrite Nat.add_assoc
-  end.
-
-Hint Extern 10 => progress unfold map_branches_k : all.
-
-Ltac solve_all_one :=
-  try lazymatch goal with
-  | H: tCasePredProp _ _ _ |- _ => destruct H
-  end;
-  unfold tCaseBrsProp, tFixProp in *;
-  try apply map_predicate_eq_spec;
-  try apply map_predicate_id_spec;
-  repeat toAll; try All_map; try close_Forall;
-  change_Sk; auto with all;
-  intuition eauto 4 with all.
-
-Ltac solve_all := repeat (progress solve_all_one).
-Hint Extern 10 => rewrite !map_branch_map_branch : all.
-Hint Extern 10 => rewrite !map_predicate_map_predicate : all.
-
 Ltac nth_leb_simpl :=
   match goal with
     |- context [leb ?k ?n] => elim (leb_spec_Set k n); try lia; simpl
