pcuic/theories/PCUICTyping.v
@@ -37,8 +37,6 @@ Fixpoint isArity T :=
   | _ => False
   end.
 
-Include PCUICLookup.
-
 Definition type_of_constructor mdecl (cdecl : ident * term * nat) (c : inductive * nat) (u : list Level.t) :=
   let mind := inductive_mind (fst c) in
   subst0 (inds mind u mdecl.(ind_bodies)) (subst_instance_constr u (snd (fst cdecl))).
